theories/Prelude/Prelude.v
@@ -21,6 +21,7 @@ Reserved Infix "=~=" (no associativity, at level 70).
 Reserved Infix "\in" (no associativity, at level 70).
 Reserved Infix "\subseteq" (no associativity, at level 70).
 Reserved Infix ">>=" (left associativity, at level 90).
+Reserved Infix "≡" (no associativity, at level 70).
 
 Module B.
 
